Porting char to the new style of Haskell theory

opentheory/haskell/char.ml
@@ -15,92 +15,68 @@ logfile "haskell-char-def";;
 
 (* Unicode characters *)
 
-let (planeH_lift_drop,planeH_drop_lift) =
-  let exists = prove (`?(p : plane). T`, REWRITE_TAC []) in
-  let tybij =
-    new_type_definition
-      "planeH" ("lift_planeH","drop_planeH") exists in
-  CONJ_PAIR (REWRITE_RULE [] tybij);;
+let planeH_tybij = define_haskell_type
+  `:plane`
+  [];;
 
-export_thm planeH_lift_drop;;
-export_thm planeH_drop_lift;;
+export_thm planeH_tybij;;
 
-let planeH_tybij = CONJ planeH_lift_drop planeH_drop_lift;;
+let positionH_tybij = define_haskell_type
+  `:position`
+  [];;
 
-let (positionH_lift_drop,positionH_drop_lift) =
-  let exists = prove (`?(p : position). T`, REWRITE_TAC []) in
-  let tybij =
-    new_type_definition
-      "positionH" ("lift_positionH","drop_positionH") exists in
-  CONJ_PAIR (REWRITE_RULE [] tybij);;
+export_thm positionH_tybij;;
 
-export_thm positionH_lift_drop;;
-export_thm positionH_drop_lift;;
+let unicodeH_tybij = define_haskell_type
+  `:unicode`
+  [];;
 
-let positionH_tybij = CONJ positionH_lift_drop positionH_drop_lift;;
+export_thm unicodeH_tybij;;
 
-let (unicodeH_lift_drop,unicodeH_drop_lift) =
-  let exists = prove (`?(p : unicode). T`, REWRITE_TAC []) in
-  let tybij =
-    new_type_definition
-      "unicodeH" ("lift_unicodeH","drop_unicodeH") exists in
-  CONJ_PAIR (REWRITE_RULE [] tybij);;
-
-export_thm unicodeH_lift_drop;;
-export_thm unicodeH_drop_lift;;
-
-let unicodeH_tybij = CONJ unicodeH_lift_drop unicodeH_drop_lift;;
-
-let mk_planeH_def = new_definition
-  `!b : byte. mk_planeH b = lift_planeH (mk_plane b)`;;
+let mk_planeH_def = define_haskell_const
+  `mk_plane : byte -> plane`;;
 
 export_thm mk_planeH_def;;
 
-let dest_planeH_def = new_definition
-  `!p : planeH. dest_planeH p = dest_plane (drop_planeH p)`;;
+let dest_planeH_def = define_haskell_const
+  `dest_plane : plane -> byte`;;
 
 export_thm dest_planeH_def;;
 
-let mk_positionH_def = new_definition
-  `!w : word16. mk_positionH w = lift_positionH (mk_position w)`;;
+let mk_positionH_def = define_haskell_const
+  `mk_position : word16 -> position`;;
 
 export_thm mk_positionH_def;;
 
-let dest_positionH_def = new_definition
-  `!p : positionH. dest_positionH p = dest_position (drop_positionH p)`;;
+let dest_positionH_def = define_haskell_const
+  `dest_position : position -> word16`;;
 
 export_thm dest_positionH_def;;
 
-let mk_unicodeH_def = new_definition
-  `!pl pos.
-      mk_unicodeH (pl,pos) =
-      lift_unicodeH (mk_unicode (drop_planeH pl, drop_positionH pos))`;;
+let mk_unicodeH_def = define_haskell_const
+  `mk_unicode : plane # position -> unicode`;;
 
 export_thm mk_unicodeH_def;;
 
-let dest_unicodeH_def = new_definition
-  `!c.
-      dest_unicodeH c =
-      let (pl,pos) = dest_unicode (drop_unicodeH c) in
-      (lift_planeH pl, lift_positionH pos)`;;
+let dest_unicodeH_def = define_haskell_const
+  `dest_unicode : unicode -> plane # position`;;
 
 export_thm dest_unicodeH_def;;
 
 (* UTF-8 encoding *)
 
+let decoder_parseH_def = define_haskell_const
+  `decoder_parse :
+   byte -> byte pstream -> (unicode # byte pstream) option`;;
+
+export_thm decoder_parseH_def;;
+
+let decoderH_def = define_haskell_const
+  `decoder : (byte,unicode) parser`;;
+
+export_thm decoderH_def;;
+
 (***
-let decoder_parseH_def = new_definition
-  `decoder_parseH =
-   lift_parser_functionH
-     (\b s. parse_map lift_unicodeH decoder)`;;
-
-export_thm decoderH_def;;
-
-let decoderH_def = new_definition
-  `decoderH = lift_parserH (parse_map lift_unicodeH decoder)`;;
-
-export_thm decoderH_def;;
-
 let decode_pstreamH_def = new_definition
   `!bs.
      decode_pstreamH bs =
@@ -113,6 +89,7 @@ export_thm decode_pstreamH_def;;
 (* Properties.                                                               *)
 (* ------------------------------------------------------------------------- *)
 
+(***
 logfile "haskell-char-thm";;
 
 (* Unicode characters *)
@@ -145,6 +122,7 @@ let unicodeH_mk_dest = prove
 export_thm unicodeH_mk_dest;;
 
 (* UTF-8 encoding *)
+***)
 
 (* ------------------------------------------------------------------------- *)
 (* Source.                                                                   *)
